coq/VarSet.v
@@ -1,0 +1,70 @@
+Require Import Coq.Unicode.Utf8_core.
+Require Import Coq.Bool.Bool.
+Require Import Coq.Arith.Arith.
+
+
+Inductive varSet : Type :=
+| Empty : varSet
+| Var   : nat -> varSet -> varSet.
+
+Fixpoint member_ (vs: varSet) (n:nat) : bool :=
+match vs with
+| Empty        => false
+| Var m rest => if (beq_nat n m) then true else member_ rest n
+end.
+
+Inductive member : varSet -> nat -> Prop :=
+| member_var : forall n rest,  member (Var n rest) n
+| member_rest : forall n1 n2 rest, not (n1 = n2) ->
+                                   member rest n1 ->
+                                   member (Var n2 rest) n2.
+
+Inductive notMember : varSet -> nat -> Prop :=
+| notMember_empty : forall n, notMember Empty n
+| notMember_var   : forall n n1 rest, not (n = n1) ->
+                                      notMember rest n ->
+                                      notMember (Var n1 rest) n.
+
+Fixpoint add_ (vs : varSet) (n: nat) : varSet :=
+  if (member_ vs n) then
+    vs
+  else
+    (Var n vs).
+
+Inductive add : varSet -> nat -> varSet -> Prop :=
+| IsMember : forall n vs, member vs n -> add vs n vs
+| IsNotMember : forall n vs, notMember vs n -> add vs n (Var n vs).
+
+Inductive unique : varSet -> Prop :=
+| unique_empty : unique Empty
+| unique_var   : forall n rest, notMember rest n ->
+                                unique rest ->
+                                unique (Var n rest).
+
+Fixpoint union_ (vs1 vs2: varSet) : varSet :=
+match vs1 with
+| Empty      => vs2
+| Var n rest => union_ rest (add_ vs2 n)
+end.
+
+Inductive union : varSet -> varSet -> varSet -> Prop :=
+| union_empty : forall vs, union Empty vs vs
+| union_var   : forall n rest vs vsInt vsRes, add vs n vsInt ->
+                                              union rest vsInt vsRes ->
+                                              union (Var n rest) vs vsRes.
+
+Theorem union_unique :
+  forall vs1 vs2 vsRes, unique vs1 ->
+                        unique vs2 ->
+                        union vs1 vs2 vsRes -> 
+                        unique vsRes.
+Proof.
+  intros vs1 vs2 vsRes Hvs1 Hvs2 Hunion.
+  induction Hunion.
+  - assumption.
+  - apply IHHunion.
+    + inversion Hvs1. subst. assumption.
+    + inversion H; subst.
+      * assumption.
+      * constructor. assumption. assumption.
+Qed. 
